\documentclass[a4paper,11pt]{article}
\usepackage{amsmath}
\begin{document}
\begin{flushright}
Matthew Olsen\\
March 23, 2016\\ 
CSE: 122 Homework 4B\\
\end{flushright}

\section{Homework 4B}
	\subsection{Problem 1}
	\textbf{Equation:}\\
	\begin{equation*}
		b_k = \frac{b_{k-1}}{1+b_{k-1}}
	\end{equation*}
	\textbf{Work for Explicit Formula}\\
	\begin{gather*}
		b_{k-1} = \frac{b_{k-2}}{1+b_{k-2}}\\
		b_k = \frac{\frac{b_{k-2}}{1+b_{k-2}}}{1 + \frac{b_{k-2}}{1+b_{k-2}}} = \frac{\frac{b_{k-2}}{1+b_{k-2}}}{\frac{1+2b_{k-2}}{1+b_{k-2}}}\\
		b_k = \frac{b_{k-2}}{1+2b_{k-1}}\\
		b_{k-2} = \frac{b_{k-3}}{1+b_{k-3}}\\
		b_k = \frac{\frac{b_{k-3}}{1+b_{k-3}}}{1 + \frac{2b_{k-3}}{1+b_{k-3}}} = \frac{\frac{b_{k-3}}{1+b_{k-3}}}{\frac{1+3b_{k-3}}{1+b_{k-3}}}\\
		b_k = \frac{b_{k-3}}{1+3b_{k-3}}\\
		b_k = \frac{b_{k-n}}{1+nb_{k-n}}\\
		b_{k-n}=b_{0} \Rightarrow k-n=0 \Rightarrow k=n\\
		b_k = \frac{b_{k-k}}{1+kb_{k-k}} = \frac{b_0}{1+k(b_0)}\\
		\mathbf{b_k=\frac{1}{1+k}}
	\end{gather*}
	\textbf{Proof by Induction}\\
	\textbf{Equation}\\
	\begin{equation*}
		b_n=\frac{b_{n-1}}{1+b_{n-1}}=\frac{1}{1+n}, \text{where $b_0 = 1$}
	\end{equation*}
	\textbf{Base Case:} If n = 0\\
	\begin{equation*}
		b_0=\frac{1}{1+0}=1
	\end{equation*}
	\textbf{Assumtpion:} If n = k, then\\
	\begin{equation*}
		b_{k}=\frac{b_{k-1}}{1+b_{k-1}}=\frac{1}{1+k}
	\end{equation*}
	\textbf{Prove:} If n = k + 1, then\\
	\begin{equation*}
		b_{k+1}=\frac{b_k}{1+b_k}=\frac{1}{2+k}
	\end{equation*}
	\textbf{Proof:}\\
	\begin{equation*}
		b_{k+1}=\frac{b_k}{1+b_k}=\frac{\frac{1}{1+k}}{1+\frac{1}{1+k}}=\frac{b_k}{1+b_k}=\frac{\frac{1}{1+k}}{\frac{2+k}{1+k}}=\frac{1}{2+k}
	\end{equation*}
	
    \subsection{Problem 2}
	\textbf{Equation:}\\
	\begin{equation*}
		T(n)=T(\frac{n}{2})+b,T(1)=a
	\end{equation*}
	\textbf{Work for Explicit Formula:}\\
	\begin{gather*}
		T(\frac{n}{2}) = T(\frac{n}{4})+b\\
		T(n)=T(\frac{n}{4})+2b\\
		T(\frac{n}{4}) = T(\frac{n}{8})+b\\
		T(n)=T(\frac{n}{8})+3b\\
		\mathbf{T(n)=T(\frac{n}{2^k})+kb}\\
		T(\frac{n}{2^k})=T(1) \Rightarrow \frac{n}{2^k}=1 \Rightarrow n = 2^k \Rightarrow log_2(n)=k\\
		T(n)=T(\frac{2^k}{2^k})+log_2(n)b\\
		\textbf{Explicit Equation: }T(n)=a+log_2(n)b\\
		\textbf{Big-O: }O(log(n))
	\end{gather*}

	\subsection{Problem 3}
	\textbf{Equation:}\\
	\begin{equation*}
		T(n)=2T(\frac{n}{2})+b,T(1)=a
	\end{equation*}
	\textbf{Work for Explicit Formula:}\\
	\begin{gather*}
		T(\frac{n}{2}) = 2T(\frac{n}{4})+b\\
		T(n)=2*(T(\frac{n}{4})+b)+b=2T(\frac{n}{4})+2b+b\\
		T(\frac{n}{4}) = 2T(\frac{n}{8})+b\\
		T(n)=8T(\frac{n}{8})+4b+2b+b\\
		\mathbf{T(n)=2^kT(\frac{n}{2^k})+2^{k-1}b}\\
		T(\frac{n}{2^k})=T(1) \Rightarrow \frac{n}{2^k}=1 \Rightarrow n = 2^k \Rightarrow log_2(n)=k\\
		T(n)=2^{log_2(n)}T(\frac{2^k}{2^k})+2^{log_2(n)-1}b\\
		\textbf{Explicit Equation: }T(n)=na+\frac{n}{2}b\\
		\textbf{Big-O: }O(n)
	\end{gather*}

	\subsection{Problem 4}
	\textbf{Equation:}\\
	\begin{equation*}
		T(n)=T(n-1)+n^k,T(1)=a
	\end{equation*}
	\textbf{Work for Explicit Formula:}\\
	\begin{gather*}
		T(n-1) = T((n-1)-1)+(n-1)^k\\
		T(n)=T(n-2)+(n-1)^k+n^k\\
		T(n-2) = T(n-3)+(n-2)^k\\
		T(n)=T(n-3)+(n-2)^k+(n-1)^k+n^k\\
		T(n-3) = T(n-4)+(n-3)^k\\
		T(n)=T(n-4)+(n-3)^k+(n-2)^k+(n-1)^k+n^k\\
		\mathbf{T(n)=T(n-j)+\sum^{j-1}_{i=0}(n-i)^k}\\
		T(n-j)=T(1)\Rightarrow n-j=1\Rightarrow j=n-1\\
		T(n)=T(n-n+1)+\sum^{(n-1)-1}_{i=0}(n-i)^k\\
		\textbf{Explicit Equation: }T(n)=a+\sum^{n-2}_{i=0}(n-i)^k\\
	\end{gather*}
	\textbf{Prove $\mathbf{T(n)=a+\sum^{n-2}_{i=0}(n-i)^k}$ is $\mathbf{O(n^{k+1})}$}
	\begin{gather*}
		a+\sum^{n-2}_{i=0}(n-i)^k=a+n^k+(n-1)^k+...+2^k\\
		< an^k+n^k+n^k+...+n^k \text{ ($n-1$ times)} = an^k + n*n^k -n^k\\
		= (a-1)n^k + n^{k+1} < a*n^{k+1}+n^{k+1}=a*n^{k+1}\\
		\mathbf{a+\sum^{n-2}_{i=0}(n-i)^k \leq a*n^{k+1}}\\
		n_0 = 1\\
		c = a\\
		\textbf{Big-O: }O(n^{k+1})\\
	\end{gather*}
\end{document}
